LeanScratch/Semantics/Conc/Red.lean
@@ -1,0 +1,50 @@
+import LeanScratch.Semantics.Conc.Stx
+import Batteries.Data.HashMap.Basic
+import Mathlib.Data.Rel
+import Mathlib.Data.List.AList
+import LeanScratch.Relation
+
+namespace L1Par
+
+abbrev VarMap := AList (fun _ : String => Int)
+abbrev MtxMap := AList (fun _ : String => Bool)
+
+abbrev State := Expr × MtxMap × VarMap
+
+inductive Red : State → State → Prop
+  | op_add (a b : Int) : Red ⟨.op (.int a) .add (.int b), s⟩ ⟨.int (a + b), s⟩
+  | op_gte (a b : Int) : Red ⟨.op (.int a) .gte (.int b), s⟩ ⟨.bool (a >= b), s⟩
+
+  | op1 : Red ⟨e, s⟩ ⟨e', s'⟩
+      → Red ⟨.op e o e2, s⟩ ⟨.op e' o e2, s'⟩
+  | op2 : Red ⟨e2, s⟩ ⟨e2', s'⟩
+      → e.IsValue → Red ⟨.op e o e2, s⟩ ⟨.op e o e2', s'⟩
+
+  | deref : (h : s.lookup addr = some x)
+      → Red ⟨.deref (addr), mtx, s⟩ ⟨.int x, mtx, s⟩
+  | assign1 : (h : ∃ x, s.lookup addr = some x)
+      → Red ⟨.assign addr (.int v), mtx, s⟩ ⟨.skip, mtx, s.insert addr v⟩
+  | assign2 : Red ⟨e, s⟩ ⟨e', s'⟩ → Red ⟨.assign addr e, s⟩ ⟨.assign addr e', s'⟩
+
+  | seq1: Red ⟨.seq .skip e, mtx, s⟩ ⟨e, mtx, s⟩
+  | seq2: Red ⟨e1, s⟩ ⟨e1', s'⟩
+      → Red ⟨.seq e1 e2, s⟩ ⟨.seq e1' e2, s'⟩
+
+  | if_t: Red ⟨.eif (.bool true) e1 e2, s⟩ ⟨e1, s⟩
+  | if_f: Red ⟨.eif (.bool false) e1 e2, s⟩ ⟨e2, s⟩
+
+  | if_cond: Red ⟨condition, s⟩ ⟨condition', s'⟩
+      → Red ⟨.eif condition e1 e2, s⟩ ⟨.eif condition' e1 e2, s'⟩
+
+  | ewhile : Red ⟨.ewhile c body, stx⟩ ⟨.eif c (.seq body (.ewhile c body)) .skip, stx⟩
+
+  | par1 : Red ⟨e, s⟩ ⟨e', s'⟩
+      → Red ⟨.par e e2, s⟩ ⟨.par e' e2, s'⟩
+  | par2 : Red ⟨e, s⟩ ⟨e', s'⟩
+      → Red ⟨.par e2 e, s⟩ ⟨.par e2 e', s'⟩
+
+  | lock : mtx.lookup nm = .some .false →
+      Red ⟨.lock nm, mtx, s⟩ ⟨.skip, mtx.insert nm .true, s⟩
+  | unlock : Red ⟨.unlock nm, mtx, s⟩ ⟨.skip, mtx.insert nm .false, s⟩
+
+
