LeanScratch/Semantics/Conc/Stx.lean
@@ -1,0 +1,38 @@
+import Mathlib.Data.Rel
+
+namespace L1Par
+
+inductive Op
+  | add
+  | gte
+
+inductive TExpr
+  | bool (val : Bool)
+  | int  (val : Int)
+
+  | op (lhs : TExpr) (op : Op) (rhs : TExpr)
+
+  | eif    (cond t f : TExpr)
+  | ewhile (cond e   : TExpr)
+
+  | assign (addr : String) (e : TExpr)
+  | deref (addr : String)
+  | seq   (a b : TExpr)
+  | skip
+
+  | lock   (name : String)
+  | unlock (name : String)
+
+inductive Expr
+  | tex (v : TExpr)
+  | par (a b : Expr)
+
+inductive TExpr.IsValue : TExpr → Prop
+  | bool : IsValue (.bool b)
+  | int  : IsValue (.int i)
+  | skip : IsValue .skip
+
+inductive Expr.IsValue : Expr → Prop
+  | tex : v.IsValue → IsValue (.tex v)
+  | par (ha : IsValue a) (hb : IsValue b) : IsValue (.par a b)
+
