LeanScratch/Semantics/Conc/Typed.lean
@@ -1,0 +1,63 @@
+import LeanScratch.Semantics.Conc.Stx
+import LeanScratch.Relation
+import Mathlib.Data.List.AList
+
+namespace L1Par
+
+inductive Ty
+  | bool
+  | int
+  | void
+  | proc
+deriving DecidableEq
+
+-- TODO: Change Int to Unit
+abbrev Ctx := AList fun _ : String => Int
+
+inductive TTySpec : Ctx → TExpr → Ty → Prop
+  | bool : TTySpec _ (.bool b) .bool
+  | int  : TTySpec _ (.int i)  .int
+  | skip : TTySpec _ .skip     .void
+
+  | op_add : TTySpec ctx a .int → TTySpec ctx b .int
+      → TTySpec ctx (.op a .add b) .int
+  | op_gte : TTySpec ctx a .int → TTySpec ctx b .int
+      → TTySpec ctx (.op a .gte b) .bool
+
+  | deref : (h : ∃ w, ctx.lookup addr = some w)
+      → TTySpec ctx (.deref addr) .int
+  | assign : (h : ∃ w, ctx.lookup addr = some w) → TTySpec ctx e .int
+      → TTySpec ctx (.assign addr e) .void
+  | seq : TTySpec ctx a .void → TTySpec ctx b o
+      → TTySpec ctx (.seq a b) o
+
+  | eif : TTySpec ctx c .bool → TTySpec ctx t a → TTySpec ctx f a
+      → TTySpec ctx (.eif c t f) a
+
+  | ewhile : TTySpec ctx c .bool → TTySpec ctx body .void
+      → TTySpec ctx (.ewhile c body) .void
+
+  | lock   (h : ∃ w, ctx.lookup addr = some w) :
+        TTySpec ctx (.lock   addr) .void
+  | unlock   (h : ∃ w, ctx.lookup addr = some w) :
+        TTySpec ctx (.unlock addr) .void
+
+theorem NonProc : ¬TTySpec ctx e .proc := fun h =>
+  match e with
+  | .bool _
+  | .int _
+  | .skip
+  | .op _ _ _
+  | .deref _
+  | .assign _ _
+  | .lock _
+  | .unlock _ => by cases h
+  | .seq _ v   => match h with | .seq _ h   => NonProc h
+  | .eif _ v _ => match h with | .eif _ h _ => NonProc h
+
+inductive TySpec : Ctx → Expr → Ty → Prop
+  | tex : TTySpec ctx e .void → TySpec ctx (.tex e) .proc
+  | parallel : TySpec ctx a .proc →
+               TySpec ctx b .proc
+      → TySpec ctx (.par a b) .proc
+
