LeanScratch/Semantics/L1Par/Red.lean
@@ -1,0 +1,83 @@
+import LeanScratch.Semantics.Conc.Stx
+import Batteries.Data.HashMap.Basic
+import Mathlib.Data.Rel
+import Mathlib.Data.List.AList
+import LeanScratch.Relation
+
+namespace L1Par
+
+abbrev VarMap := AList (fun _ : String => Int)
+abbrev MtxMap := AList (fun _ : String => Bool)
+
+inductive Act
+  | tau
+  | ass (addr : String) (v : Int)
+  | drf (addr : String) (v : Int)
+  | lock (addr : String)
+  | unlock (addr : String)
+
+inductive TLRed : TExpr → TExpr → Act → Prop
+  | op_add : TLRed (.op (.int a) .add (.int b)) (.int (a + b)) .tau
+  | op_gte : TLRed (.op (.int a) .gte (.int b)) (.bool (a >= b)) .tau
+
+  | op1 : TLRed a a' act
+      → TLRed (.op a op b) (.op a' op b) act
+  | op2 : b.IsValue → TLRed a a' act
+      → TLRed (.op b op a) (.op b op a') act
+
+  | deref : TLRed (.deref l) (.int v) (.drf l v)
+  | ass1  : TLRed (.assign l (.int v)) .skip (.ass l v)
+  | ass2  : TLRed a a' act
+      → TLRed (.assign l a) (.assign l a') act
+
+  | seq1  : TLRed (.seq .skip a) a .tau
+  | seq2  : TLRed a a' act → TLRed (.seq a b) (.seq a' b) act
+
+  | if_t : TLRed (.eif (.bool .true) a b)  a .tau
+  | if_f : TLRed (.eif (.bool .false) a b) b .tau
+  | if_cond : TLRed a a' act
+      → TLRed (.eif a t f) (.eif a' t f) act
+
+  | ewhile : TLRed (.ewhile c body) (.eif c (.seq body $ .ewhile c body) .skip) .tau
+
+  | lock   : TLRed (.lock   s) .skip (.lock   s)
+  | unlock : TLRed (.unlock s) .skip (.unlock s)
+
+inductive GRed : Expr → VarMap → MtxMap → Expr → VarMap → MtxMap → Prop
+  | tau    : TLRed e e' .tau
+      → GRed (.tex e) store mtx (.tex e') store mtx
+  | drf    : TLRed e e' (.drf addr n) → store.lookup addr = .some n
+      → GRed (.tex e) store mtx (.tex e') store mtx
+  | ass    : TLRed e e' (.ass addr n)
+      → GRed (.tex e) store mtx (.tex e') (store.insert addr n) mtx
+  | lock   : TLRed e e' (.lock addr) → mtx.lookup addr = .some .false
+      → GRed (.tex e) store mtx (.tex e') store (mtx.insert addr .true)
+  | unlock : TLRed e e' (.unlock addr)
+      → GRed (.tex e) store mtx (.tex e') store (mtx.insert addr .false)
+
+  | par1 : GRed a ctx mtx a' ctx' mtx'
+      → GRed (.par a b) ctx mtx (.par a' b) ctx' mtx'
+  | par2 : GRed a ctx mtx a' ctx' mtx'
+      → GRed (.par b a) ctx mtx (.par b a') ctx' mtx'
+
+def Expr.paralize : Expr → List TExpr
+  | .par a b => a.paralize ++ b.paralize
+  | .tex v   => [v]
+
+inductive TParRed : List TExpr → VarMap → MtxMap → List TExpr → VarMap → MtxMap → Prop
+  | tau    : TLRed e e' .tau
+      → TParRed (e :: tl) store mtx (e' :: tl) store mtx
+  | drf    : TLRed e e' (.drf addr n) → store.lookup addr = .some n
+      → TParRed (e :: tl) store mtx (e' :: tl) store mtx
+  | ass    : TLRed e e' (.ass addr n)
+      → TParRed (e :: tl) store mtx (e' :: tl) (store.insert addr n) mtx
+  | lock   : TLRed e e' (.lock addr) → mtx.lookup addr = .some .false
+      → TParRed (e :: tl) store mtx (e' :: tl) store (mtx.insert addr .true)
+  | unlock : TLRed e e' (.unlock addr)
+      → TParRed (e :: tl) store mtx (e' :: tl) store (mtx.insert addr .false)
+
+  | par    : TParRed tl ctx mtx tl' ctx' mtx'
+      → TParRed (e :: tl) ctx mtx (e :: tl') ctx' mtx'
+
+
+
