LeanScratch/Semantics/LSub/Stx.lean
@@ -1,0 +1,27 @@
+inductive Ty
+  | int
+  | record : List Ty → Ty
+  | fn : Ty → Ty → Ty
+
+inductive PairWise (R : α → β → Prop) : List α → List β → Prop
+  | nil : PairWise R [] []
+  | cons : R a b → PairWise R as bs → PairWise R (a :: as) (b :: bs)
+
+inductive TySub : Ty → Ty → Prop
+  | int : TySub .int .int
+  | fn (arg : TySub b1 a1) (ret : TySub a2 b2) :
+    TySub (.fn a1 a2) (.fn b1 b2)
+  | record :
+    PairWise TySub as bs →
+    TySub (.record as) (.record bs)
+
+theorem TySub.refl : TySub a a := 
+  match a with
+  | .int => .int
+  | .fn a b => .fn TySub.refl TySub.refl
+  | .record vs => 
+    let rec x vs : PairWise TySub vs vs := match vs with
+      | [] => .nil
+      | hd :: tl => .cons TySub.refl (x tl)
+    .record (x vs)
+
