LeanScratch/Semantics/SemEquiv/Basic.lean
@@ -1,0 +1,22 @@
+import LeanScratch.Semantics.L1.Red
+
+namespace L1
+
+
+/-
+  In L3, due to scoping of contexts, then semantic equivalence is very
+  hard to figure out do to how varaibles are scoped.
+
+  The big key here is the requirement of a context C[_].
+-/
+
+inductive CC (R : α → α → Prop) : ℕ → α → α → Prop
+  | base : CC R 0 a a
+  | cont : CC R n a b → R b c → CC R n.succ a c
+
+theorem LoopPerm (hlt : n > 0) (x : CC R n a a) : ∀ k, ∃ z, CC R k a z := by
+  intro k
+  induction k
+  · exact ⟨_, .base⟩
+  · sorry
+
